Refactoring CommandEval arguments.
Was too eager when I earlier made many of the arguments to the relation implicit.  Since Imp is imperative and has mutable state, the definition of equivalence between programs often comes down to 'produces the same global state'.  Accordingly, several theorems require explicit manipulation states, which was painful when they were implicit arguments.

Refactored to make the state arguments explicit but left the other non-hypothesis arguments implicit.  Also, moved the state arguments to immediately follow the implicit arguments for consistency.  Now, if you have to use the '@' syntax to include all arguments, you only have to inject fields at the beginning, not in the middle, of the pattern.

SoftwareFoundations/LogicalFoundations/Imp.lean
@@ -506,19 +506,19 @@ def Command.noBueno (state: State): Command → State
 -/
 
 inductive CommandEval: Command → State → State → Prop where
-  | skip {s: State}: CommandEval .skip s s
-  | assign {s: State} {e: Arith} {n: Nat} {id: String} (h: e.eval s = n): CommandEval (.assign id e) s (s.update id n)
-  | seq {c₁ c₂: Command} {s₁ s₂ s₃: State} (h₁: CommandEval c₁ s₁ s₂) (h₂: CommandEval c₂ s₂ s₃): CommandEval (.seq c₁ c₂) s₁ s₃
-  | ifTrue {s₁ s₂: State} {c: Logic} {t f: Command} (h₁: c.eval s₁ = .true) (h₂: CommandEval t s₁ s₂): CommandEval (.if c t f) s₁ s₂
-  | ifFalse {s₁ s₂: State} {c: Logic} {t f: Command} (h₁: c.eval s₁ = .false) (h₂: CommandEval f s₁ s₂): CommandEval (.if c t f) s₁ s₂
-  | whileTrue {s₁ s₂ s₃: State} {c: Logic} {b: Command} (h₁: c.eval s₁ = .true) (h₂: CommandEval b s₁ s₂) (h₃: CommandEval (.while c b) s₂ s₃): CommandEval (.while c b) s₁ s₃
-  | whileFalse {c: Logic} {s: State} {b: Command} (h₁: c.eval s = .false): CommandEval (.while c b) s s
+  | skip (s: State): CommandEval .skip s s
+  | assign {e: Arith} {n: Nat} {id: String} (s: State) (h: e.eval s = n): CommandEval (.assign id e) s (s.update id n)
+  | seq {c₁ c₂: Command} (s₁ s₂ s₃: State) (h₁: CommandEval c₁ s₁ s₂) (h₂: CommandEval c₂ s₂ s₃): CommandEval (.seq c₁ c₂) s₁ s₃
+  | ifTrue {c: Logic} {t f: Command} (s₁ s₂: State) (h₁: c.eval s₁ = .true) (h₂: CommandEval t s₁ s₂): CommandEval (.if c t f) s₁ s₂
+  | ifFalse {c: Logic} {t f: Command} (s₁ s₂: State) (h₁: c.eval s₁ = .false) (h₂: CommandEval f s₁ s₂): CommandEval (.if c t f) s₁ s₂
+  | whileTrue {c: Logic} {b: Command} (s₁ s₂ s₃: State) (h₁: c.eval s₁ = .true) (h₂: CommandEval b s₁ s₂) (h₃: CommandEval (.while c b) s₂ s₃): CommandEval (.while c b) s₁ s₃
+  | whileFalse {c: Logic} {b: Command} (s: State) (h₁: c.eval s = .false): CommandEval (.while c b) s s
 
 def assignment (id: String) (n: Nat) (s: State): CommandEval (Command.assign id (n: Arith)) s (s.update id n) :=
     have h: (n: Arith).eval s = n := by
       unfold Arith.eval
       rfl
-    CommandEval.assign h
+    CommandEval.assign s h
 
 section
   /- Useful definitions to save typing -/
@@ -548,11 +548,11 @@ section
         unfold Logic.eval
         rfl
       have h₂: CommandEval z4 s₂ s₃ := assignment "Z" 4 s₂
-      CommandEval.ifFalse h₁ h₂
+      CommandEval.ifFalse s₂ s₃ h₁ h₂
 
     by
       repeat unfold instCoeListCommand.conv
-      exact CommandEval.seq h₁ h₂
+      exact CommandEval.seq s₁ s₂ s₃ h₁ h₂
 
   /- x := 0; y := 1; z := 2 -/
   example: CommandEval [x0, y1, z2] State.empty (State.build [("X", 0), ("Y", 1), ("Z", 2)]) :=
@@ -589,7 +589,7 @@ theorem CommandEval.deterministic (c: Command) (s₁ s₂ s₃: State) (h₁: Co
 
 example (s₁ s₂: State) (n: Nat) (h₁: s₁ "X" = n) (h₂: CommandEval plus2 s₁ s₂): s₂ "X" = n + 2 := by
   cases h₂ with
-    | assign h =>
+    | assign _ h =>
       simp
       repeat unfold Arith.eval at h
       rw [h₁] at h
@@ -598,7 +598,7 @@ example (s₁ s₂: State) (n: Nat) (h₁: s₁ "X" = n) (h₂: CommandEval plus
 
 example (s₁ s₂: State) (n₁ n₂: Nat) (h₁: s₁ "X" = n₁) (h₂: s₁ "Y" = n₂) (h₃: CommandEval xTimesYInZ s₁ s₂): s₂ "Z" = n₁ * n₂ := by
   cases h₃ with
-    | assign h =>
+    | assign _ h =>
       repeat unfold Arith.eval at h
       repeat unfold Arith.eval at h
       rw [h₁, h₂] at h
@@ -708,14 +708,14 @@ namespace BreakImp
     | break: Result
 
   inductive CommandEval: Command → State → Result → State → Prop where
-    | skip (state: State): CommandEval .skip state .continue state
-    | break (state: State): CommandEval .break state .break state
-    | assign (state: State) (e: Arith) (n: Nat) (id: String) (h: e.eval state = n): CommandEval (.assign id e) state .continue (state.update id n)
-    | seq (c₁ c₂: Command) (s₁ s₂ s₃: State) (h₁: CommandEval c₁ s₁ .continue s₂) (h₂: CommandEval c₂ s₂ .continue s₃): CommandEval (.seq c₁ c₂) s₁ .continue s₃
-    | ifTrue (s₁ s₂: State) (c: Logic) (t f: Command) (h₁: c.eval s₁ = .true) (h₂: CommandEval t s₁ .continue s₂): CommandEval (.if c t f) s₁ .continue s₂
-    | ifFalse (s₁ s₂: State) (c: Logic) (t f: Command) (h₁: c.eval s₁ = .false) (h₂: CommandEval f s₁ .continue s₂): CommandEval (.if c t f) s₁ .continue s₂
-    | whileTrue (s₁ s₂ s₃: State) (c: Logic) (b: Command) (h₁: c.eval s₁ = .true) (h₂: CommandEval b s₁ .continue s₂) (h₃: CommandEval (.while c b) s₂ .continue s₃): CommandEval (.while c b) s₁ .continue s₃
-    | whileFalse (c: Logic) (s: State) (b: Command) (h₁: c.eval s = .false): CommandEval (.while c b) s .continue s
+    | skip (s: State): CommandEval .skip s .continue s
+    | break (s: State): CommandEval .break s .break s
+    | assign {e: Arith} {n: Nat} {id: String} (s: State) (h: e.eval s = n): CommandEval (.assign id e) s .continue (s.update id n)
+    | seq {c₁ c₂: Command} (s₁ s₂ s₃: State) (h₁: CommandEval c₁ s₁ .continue s₂) (h₂: CommandEval c₂ s₂ .continue s₃): CommandEval (.seq c₁ c₂) s₁ .continue s₃
+    | ifTrue {c: Logic} {t f: Command} (s₁ s₂: State) (h₁: c.eval s₁ = .true) (h₂: CommandEval t s₁ .continue s₂): CommandEval (.if c t f) s₁ .continue s₂
+    | ifFalse {c: Logic} {t f: Command} (s₁ s₂: State) (h₁: c.eval s₁ = .false) (h₂: CommandEval f s₁ .continue s₂): CommandEval (.if c t f) s₁ .continue s₂
+    | whileTrue {c: Logic} {b: Command} (s₁ s₂ s₃: State) (h₁: c.eval s₁ = .true) (h₂: CommandEval b s₁ .continue s₂) (h₃: CommandEval (.while c b) s₂ .continue s₃): CommandEval (.while c b) s₁ .continue s₃
+    | whileFalse {c: Logic} {b: Command} (s: State) (h₁: c.eval s = .false): CommandEval (.while c b) s .continue s
 
   example (c: Command) (s₁ s₂: State) (r: Result): CommandEval (.seq .break c) s₁ r s₂ := by
     sorry
